theories/Core/SubKTree.v
@@ -1,4 +1,3 @@
-Set Universe Polymorphism.
 (* begin hide *)
 From ITree Require Import
      Basics.Basics
@@ -14,126 +13,147 @@ From Coq Require Import
 
 Import CatNotations.
 Local Open Scope cat_scope.
+
+Set Universe Polymorphism.
 (* end hide *)
 
 (* We consider the transport of the symmetric traced monoidal structure of [ktree]s to a subcategory *)
 
-Class Embedding (i: Type): Type :=
-  F: i -> Type.
+Class Embedding@{uI uJ} (i : Type@{uI}): Type :=
+  F: i -> Type@{uJ}.
 
-Class Embedded_initial `{Embedding} (iI: i) :=
+Class Embedded_initial@{uI uJ} `{Embedding@{uI uJ}} (iI: i) :=
   {
     iI_void: F iI -> void;
     void_iI: void -> F iI
   }.
 
-Class Embedded_sum `{Embedding} (isum: i -> i -> i) :=
+Class Embedded_sum@{uI uJ} `{Embedding@{uI uJ}} (isum: i -> i -> i) :=
   {
     isum_sum: forall {A B: i}, F (isum A B) -> (F A) + (F B);
     sum_isum: forall {A B: i}, (F A) + (F B) -> F (isum A B)
   }.
 
+(** * Subcategories of [Fun] *)
+Section iFun.
+
+Universe uI uJ uY.
+(* We consider a subdomain of Type given by a Type [i] and its injection [F] into [Type] *)
+Context {i: Type@{uI}}.
+Context {iEmbed: Embedding@{uI uJ} i}.
+(* We assume that we have an initial element and a bifunctor over i *)
+Context {iI: i}.
+Context {isum: i -> i -> i}.
+Context {FInit: Embedded_initial iI}.
+Context {iI_iso: Iso@{uY uJ} Fun iI_void void_iI}.
+Context {Fsum: Embedded_sum isum}.
+Context {sum_Iso: forall A B, Iso@{uY uJ} Fun (@isum_sum _ _ _ _ A B) sum_isum}.
+
+(* The embedding [F] defines a subcategory of [Fun] *)
+Definition iFun (a b: i) := F a -> F b.
+
+Global Instance Eq2_iFun : Eq2 iFun :=
+  fun a b => @eq2@{uY _} _ Fun _ (F a) (F b).
+
+Global Instance Id_iFun : Id_ iFun :=
+  fun a => @id_@{uY _} _ Fun _ (F a).
+
+(** Function composition *)
+Global Instance Cat_iFun : Cat iFun :=
+  fun a b c f g => @cat@{uY _} _ Fun _ _ _ _ f g.
+
+(** [void] as an initial object. *)
+Global Instance Initial_iI : Initial iFun iI :=
+  fun a => cat@{uY _} iI_void empty@{uY uJ}.
+
+(** ** The [sum] coproduct. *)
+
+(** Coproduct elimination *)
+Global Instance case_isum : CoprodCase iFun isum :=
+  fun {a b c} f g =>  isum_sum >>> @case_@{uY _} _ Fun _ _ _ _ _ f g.
+
+(** Injections *)
+Global Instance isum_inl : CoprodInl iFun isum := fun a b => @inl_@{uY _} _ Fun _ _ _ (F b) >>> sum_isum .
+Global Instance isum_inr : CoprodInr iFun isum := fun a b => @inr_@{uY _} _ Fun _ _ _ (F a) >>> sum_isum .
+
+End iFun.
+
+(** * Subcategories of [ktree] *)
 Section SubK.
 
-  (* We consider a subdomain of Type given by a Type [i] and its injection [F] into [Type] *)
-  Context {i: Type}.
-  Context {iEmbed: Embedding i}.
-  (* We assume that we have an initial element and a bifunctor over i *)
-  Context {iI: i}.
-  Context {isum: i -> i -> i}.
-  Context {FInit: Embedded_initial iI}.
-  Context {iI_iso: Iso Fun iI_void void_iI}.
-  Context {Fsum: Embedded_sum isum}.
-  Context {sum_Iso: forall A B, Iso Fun (@isum_sum _ _ _ _ A B) sum_isum}.
+Universe uI uE uF uR uT uY.
 
-  Section iFun.
+(* We consider a subdomain of Type given by a Type [i] and its injection [F] into [Type] *)
+Context {i: Type@{uI}}.
+Context {iEmbed: Embedding@{uI uR} i}.
+(* We assume that we have an initial element and a bifunctor over i *)
+Context {iI: i}.
+Context {isum: i -> i -> i}.
+Context {FInit: Embedded_initial iI}.
+Context {iI_iso: Iso@{uY uR} Fun iI_void void_iI}.
+Context {Fsum: Embedded_sum isum}.
+Context {sum_Iso: forall A B, Iso@{uY uR} Fun (@isum_sum _ _ _ _ A B) sum_isum}.
 
-    (* The embedding [F] defines a subcategory of [Fun] *)
-    Definition iFun (a b: i) := F a -> F b.
+(* The embedding [F] defines a subcategory of [ktree] *)
+Definition sktree (E: Type@{uE} -> Type@{uF}) (A B: i) : Type@{uT}
+  := F A -> itree@{uE uF uR uT} E (F B).
 
-    Global Instance Eq2_iFun : Eq2 iFun :=
-      fun a b => @eq2 _ Fun _ (F a) (F b).
+(** ** Categorical operations *)
 
-    Global Instance Id_iFun : Id_ iFun :=
-      fun a => @id_ _ Fun _ (F a).
+Section Operations.
 
-    (** Function composition *)
-    Global Instance Cat_iFun : Cat iFun :=
-      fun a b c f g => @cat _ Fun _ _ _ _ f g. 
+Context {E : Type@{uE} -> Type@{uF}}.
 
-    (** [void] as an initial object. *)
-    Global Instance Initial_iI : Initial iFun iI :=
-      fun a => iI_void >>> empty.
+Let sktree := sktree E.
 
-    (** ** The [sum] coproduct. *)
+(* Utility function to lift a pure ([iFun]) computation into sktree *)
+Definition lift_sktree {A B: i} (f : F A -> F B) : sktree A B := lift_ktree f.
+Definition iI_voidl : ktree@{uR uT} E (F iI) void := lift_ktree_ E _ _ iI_void.
+Definition void_iIl : ktree@{uR uT} E void (F iI) := lift_ktree_ E _ _ void_iI.
 
-    (** Coproduct elimination *)
-    Global Instance case_isum : CoprodCase iFun isum :=
-      fun {a b c} f g =>  isum_sum >>> @case_ _ Fun _ _ _ _ _ f g.
+Definition isum_suml {A B : i}
+  : ktree@{uR uT} E (F (isum A B)) (sum (F A) (F B))
+  := lift_ktree_ E _ _ (@isum_sum _ _ _ _ A B).
+Definition sum_isuml {A B : i}
+  : ktree@{uR uT} E (sum (F A) (F B)) (F (isum A B))
+  := lift_ktree_ E _ _ (@sum_isum _ _ _ _ A B).
 
-    (** Injections *)
-    Global Instance isum_inl : CoprodInl iFun isum := fun a b => @inl_ _ Fun _ _ _ (F b) >>> sum_isum .
-    Global Instance isum_inr : CoprodInr iFun isum := fun a b => @inr_ _ Fun _ _ _ (F a) >>> sum_isum .
+(** *** Category *)
 
-  End iFun.
+Definition eutt_sktree {A B} (d1 d2 : sktree A B) : Prop
+  := @eq2@{uY _} _ (ktree E) _ _ _ d1 d2.
+Global Instance Eq2_sktree : Eq2 sktree := @eutt_sktree.
 
-  (* The embedding [F] defines a subcategory of [ktree] *)
-  Definition sktree (E: Type -> Type) (A B: i) := F A -> itree E (F B).
+(** Composition *)
+Global Instance Cat_sktree : Cat sktree :=
+  fun (A B C: i) (k: ktree E (F A) (F B)) (k': ktree E (F B) (F C)) =>
+    @cat@{uY _} Type@{uR} _ _ _ _ _ k k': ktree E _ _.
 
-  (** ** Categorical operations *)
+(** Identity morphism *)
+Global Instance Id_sktree : Id_ sktree :=
+  fun A => id_@{uY _} (F A).
 
-  Section Operations.
+(** *** Symmetric monoidal category *)
 
-    Context {E : Type -> Type}.
+(** Initial object, monoidal unit *)
+Global Instance Initial_iI_sktree : Initial@{uI uT} sktree iI :=
+  fun A => cat@{uY _} iI_voidl empty@{uY _}.
 
-    Let sktree := sktree E.
+(** The tensor product is given by the coproduct *)
+Global Instance Case_sktree : @CoprodCase@{uI uT} i sktree isum :=
+  fun (a b c: i) (ska: ktree _ _ _) skb => cat@{uY _} isum_suml (case_@{uY _} ska skb).
 
-    (* Utility function to lift a pure ([iFun]) computation into sktree *)
-    Definition lift_sktree {A B: i} (f : F A -> F B) : sktree A B := lift_ktree f. 
+Global Instance Inl_sktree : CoprodInl sktree isum :=
+  fun _ _ => cat@{uY _} inl_@{uY _} sum_isuml.
 
-    Definition iI_voidl {E} := lift_ktree_ E _ _ iI_void.
-    Definition void_iIl {E} := lift_ktree_ E _ _ void_iI.
+Global Instance Inr_sktree : CoprodInr sktree isum :=
+  fun _ _ => cat@{uY _} inr_@{uY _} sum_isuml.
 
-    Definition isum_suml {E A B} := lift_ktree_ E _ _ (@isum_sum _ _ _ _ A B).
-    Definition sum_isuml {E A B} := lift_ktree_ E _ _ (@sum_isum _ _ _ _ A B).
-    
-    (** *** Category *)
+Global Instance Iter_sktree : Iter sktree isum :=
+  fun A B (f : ktree E (F A) (F (isum A B))) =>
+    iter@{uY _} (cat@{uY _} f isum_suml) : ktree E (F A) (F B).
 
-    
-    Definition eutt_sktree {A B} (d1 d2 : sktree A B) := @eq2 _ (ktree E) _ _ _ d1 d2.
-    Global Instance Eq2_sktree : Eq2 sktree := @eutt_sktree.
-
-    
-    (** Composition *)
-    Global Instance Cat_sktree : Cat sktree :=
-      fun (A B C: i) (k: ktree E (F A) (F B)) (k': ktree E (F B) (F C)) => cat k k': ktree E _ _.
-
-    (** Identity morphism *)
-    Global Instance Id_sktree : Id_ sktree :=
-      fun A => id_ (F A). 
-
-    (** *** Symmetric monoidal category *)
-
-    (** Initial object, monoidal unit *)
-
-    Global Instance Initial_iI_sktree : Initial sktree iI :=
-      fun A => iI_voidl >>> empty.
-
-    (** The tensor product is given by the coproduct *)
-    Global Instance Case_sktree : @CoprodCase i sktree isum :=
-      fun (a b c: i) (ska: ktree _ _ _) skb => isum_suml >>> case_ ska skb.
-
-    Global Instance Inl_sktree : CoprodInl sktree isum :=
-      fun _ _ => inl_ >>> sum_isuml.
-
-    Global Instance Inr_sktree : CoprodInr sktree isum :=
-      fun _ _ => inr_ >>> sum_isuml.
-
-    Global Instance Iter_sktree : Iter sktree isum :=
-      fun A B (f : ktree E (F A) (F (isum A B))) =>
-        iter (f >>> isum_suml) : ktree E (F A) (F B).
-
-  End Operations.
+End Operations.
 
 End SubK.
 
