theories/Indexed/Function.v
@@ -1,4 +1,3 @@
-Set Universe Polymorphism.
 (** * The Category of Indexed Functions *)
 
 (** Indexed functions have type [E ~> F], i.e., [forall T, E T -> F T],
@@ -16,36 +15,41 @@ Set Universe Polymorphism.
 (* end hide *)
 
 (** The name of the category. *)
-Definition IFun (E F : Type -> Type) : Type := E ~> F.
+Definition IFun@{u v} (E F : Type@{u} -> Type@{v}) : Type@{max(u+1,v)}
+  := forall T : Type@{u}, E T -> F T.
+
+Definition mk_IFun@{u v} {E F : Type@{u} -> Type@{v}}
+  : (E ~> F) -> IFun@{u v} E F
+  := fun x => x.
 
 (** Unwrap [IFun], potentially useful for type inference. *)
-Definition apply_IFun {E F T} (f : IFun E F) : E T -> F T := f T.
+Definition apply_IFun@{u v} {E F T} (f : IFun@{u v} E F) : E T -> F T := f T.
 
 (** Equivalence of indexed functions is extensional equality. *)
-Instance Eq2_IFun : Eq2 IFun :=
+Instance Eq2_IFun@{u v uY uZ} : Eq2@{uY uZ} IFun@{u v} :=
   fun E F => i_pointwise (fun T => @eq (F T)).
 
 (** The identity function. *)
-Instance Id_IFun : Id_ IFun :=
+Instance Id_IFun@{u v uY uZ} : Id_@{uY uZ} IFun@{u v} :=
   fun E _ e => e.
 
 (** Function composition. *)
-Instance Cat_IFun : Cat IFun :=
+Instance Cat_IFun@{u v uY uZ} : Cat@{uY uZ} IFun@{u v} :=
   fun E F G f1 f2 R e => f2 _ (f1 _ e).
 
 (** [void1] is the initial object. *)
-Instance Initial_void1 : Initial IFun void1 :=
+Instance Initial_void1@{u v uY uZ} : Initial@{uY uZ} IFun@{u v} void1@{u v} :=
   fun _ _ v => match v : void1 _ with end.
 
 (** The coproduct is case analysis on sums. *)
-Definition case_sum1 {A B C : Type -> Type} (f : A ~> C) (g : B ~> C)
-  : A +' B ~> C
+Definition case_sum1@{u v} {A B C : Type@{u} -> Type@{v}} (f : A ~> C) (g : B ~> C)
+  : sum1@{u v} A B ~> C
   := fun _ ab =>
        match ab with
        | inl1 a => f _ a
        | inr1 b => g _ b
        end.
 
-Instance Case_sum1 : CoprodCase IFun sum1 := @case_sum1.
-Instance Inl_sum1 : CoprodInl IFun sum1 := @inl1.
-Instance Inr_sum1 : CoprodInr IFun sum1 := @inr1.
+Instance Case_sum1@{u v uY uZ} : CoprodCase@{uY uZ} IFun@{u v} sum1 := @case_sum1.
+Instance Inl_sum1@{u v uY uZ} : CoprodInl@{uY uZ} IFun@{u v} sum1 := @inl1.
+Instance Inr_sum1@{u v uY uZ} : CoprodInr@{uY uZ} IFun@{u v} sum1 := @inr1.
