theories/Events/Writer.v
@@ -1,4 +1,3 @@
-Set Universe Polymorphism.
 (** * Writer *)
 
 (** Output events. *)
@@ -21,16 +20,20 @@ From ITree Require Import
      Basics.CategoryOps
      Core.ITreeDefinition
      Indexed.Sum
+     Indexed.Function
      Core.Subevent
      Interp.Interp
      Interp.Handler
      Events.State.
 
 Import Basics.Basics.Monads.
+
+Set Universe Polymorphism.
+Set Printing Universes.
 (* end hide *)
 
 (** Event to output values of type [W]. *)
-Variant writerE (W : Type) : Type -> Type :=
+Variant writerE@{uE uF} (W : Type@{uE}) : Type@{uE} -> Type@{uF} :=
 | Tell : W -> writerE W unit.
 
 (** Output action. *)
@@ -40,16 +43,18 @@ Definition tell {W E} `{writerE W -< E} : W -> itree E unit :=
 (** One interpretation is to accumulate outputs in a list. *)
 
 (** Note that this handler appends new outputs to the front of the list. *)
-Definition handle_writer_list {W E}
-  : writerE W ~> stateT (list W) (itree E)
+Definition handle_writer_list@{uE uF uR uT} {W E}
+  : writerE@{uE uF} W ~> stateT (list W) (itree@{uE uF uR uT} E)
   := fun _ e s =>
        match e with
        | Tell w => Ret (w :: s, tt)
        end.
 
-Definition run_writer_list_state {W E}
+Definition run_writer_list_state@{uE uF uR uT uY u0 u1} {W : Type@{uE}} {E : Type@{uE} -> Type@{uF}}
   : itree (writerE W +' E) ~> stateT (list W) (itree E)
-  := interp_state (case_ handle_writer_list pure_state).
+  := interp_state@{uE uF uR uT u0 u1}
+       (case_@{uY uT} (mk_IFun handle_writer_list@{_ _ uR uT})
+                      (mk_IFun pure_state@{_ _ uR uT})).
 
 Arguments run_writer_list_state {W E} [T].
 
@@ -65,17 +70,19 @@ Arguments run_writer_list {W E} [T].
 
 (** When [W] is a monoid, we can also use that to append the outputs together. *)
 
-Definition handle_writer {W E} (Monoid_W : Monoid W)
-  : writerE W ~> stateT W (itree E)
+Definition handle_writer@{uE uF uR uT} {W E} (Monoid_W : Monoid W)
+  : writerE@{uE uF} W ~> stateT W (itree@{uE uF uR uT} E)
   := fun _ e s =>
        match e with
-       | Tell w => Ret (monoid_plus Monoid_W s w, tt) 
+       | Tell w => Ret (monoid_plus@{uE} Monoid_W s w, tt)
        end.
 
-Definition run_writer {W E} (Monoid_W : Monoid W)
+Definition run_writer@{uE uF uR uT uY u0 u1} {W E} (Monoid_W : Monoid W)
   : itree (writerE W +' E) ~> writerT W (itree E)
   := fun _ t =>
-       interp_state (case_ (handle_writer Monoid_W) pure_state) t
-                    (monoid_unit Monoid_W).
+       interp_state@{uE uF uR uT u0 u1}
+         (case_@{uY uT} (mk_IFun (handle_writer@{_ _ uR uT} Monoid_W))
+                        (mk_IFun pure_state@{_ _ uR uT})) t
+         (monoid_unit Monoid_W).
 
 Arguments run_writer {W E} Monoid_W [T].
